@prefix : <http://ontology.show-catalog.org/show#/> .
@prefix owl: <http://www.w3.org/2002/07/owl#> .
@prefix rdf: <http://www.w3.org/1999/02/22-rdf-syntax-ns#> .
@prefix xml: <http://www.w3.org/XML/1998/namespace> .
@prefix xsd: <http://www.w3.org/2001/XMLSchema#> .
@prefix rdfs: <http://www.w3.org/2000/01/rdf-schema#> .
@base <http://ontology.show-catalog.org/show#/> .

<http://ontology.show-catalog.org/show#> rdf:type owl:Ontology .

#################################################################
#    Object Properties
#################################################################

###  http://ontology.show-catalog.org/show#Knows
:Knows rdf:type owl:ObjectProperty ;
       rdfs:domain :Person ;
       rdfs:range :Person ;
       rdfs:comment "Two persons know each other if they have participated in the same show."@en ,
                    "Two persons know each other if they have participated in the same show." ;
       rdfs:label "knows"@en ,
                  "knows" .


###  http://ontology.show-catalog.org/show#/Acted_in
:Acted_in rdf:type owl:ObjectProperty ;
          rdfs:subPropertyOf :Participed_in ;
          owl:inverseOf :HasAsActor ;
          rdf:type owl:AsymmetricProperty ,
                   owl:IrreflexiveProperty ;
          rdfs:domain :Actor ;
          rdfs:range :Show ;
          rdfs:comment "Specifies a show in which an actor has performed a role"@en ,
                       "Specifies a show in which an actor has performed a role" ;
          rdfs:label "acted in"@en ,
                     "acted in" .


###  http://ontology.show-catalog.org/show#/Directed
:Directed rdf:type owl:ObjectProperty ;
          rdfs:subPropertyOf :Participed_in ;
          owl:inverseOf :HasAsDirector ;
          rdf:type owl:AsymmetricProperty ,
                   owl:IrreflexiveProperty ;
          rdfs:domain :Director ;
          rdfs:range :Show ;
          rdfs:comment "Specifies a show that a director has directed."@en ,
                       "Specifies a show that a director has directed." ;
          rdfs:label "directed"@en ,
                     "directed" .


###  http://ontology.show-catalog.org/show#/HasAsActor
:HasAsActor rdf:type owl:ObjectProperty ;
            rdfs:subPropertyOf :HasAsParticipant ;
            rdf:type owl:AsymmetricProperty ,
                     owl:IrreflexiveProperty ;
            rdfs:domain :Show ;
            rdfs:range :Actor ;
            rdfs:comment "Specifies an actor who is associated with a particular show."@en ,
                         "Specifies an actor who is associated with a particular show." ;
            rdfs:label "has as actor"@en ,
                       "has as actor" .


###  http://ontology.show-catalog.org/show#/HasAsDirector
:HasAsDirector rdf:type owl:ObjectProperty ;
               rdfs:subPropertyOf :HasAsParticipant ;
               rdf:type owl:AsymmetricProperty ,
                        owl:IrreflexiveProperty ;
               rdfs:domain :Show ;
               rdfs:range :Director ;
               rdfs:comment "Indicates the director of a particular show."@en ,
                            "Indicates the director of a particular show." ;
               rdfs:label "has as director"@en ,
                          "has as director" .


###  http://ontology.show-catalog.org/show#/HasAsParticipant
:HasAsParticipant rdf:type owl:ObjectProperty ;
                  owl:inverseOf :Participed_in ;
                  rdf:type owl:AsymmetricProperty ,
                           owl:IrreflexiveProperty ;
                  rdfs:domain :Show ;
                  rdfs:range :Person ;
                  rdfs:comment "Indicates a person who is involved in a show in any capacity, such as acting, directing, producing, etc."@en ,
                               "Indicates a person who is involved in a show in any capacity, such as acting, directing, producing, etc." ;
                  rdfs:label "has as participant"@en ,
                             "has as participant" .


###  http://ontology.show-catalog.org/show#/Has_genre
:Has_genre rdf:type owl:ObjectProperty ,
                    owl:AsymmetricProperty ,
                    owl:IrreflexiveProperty ;
           rdfs:domain :Show ;
           rdfs:range :Genre ;
           rdfs:comment "Specifies the genre or category of a show, indicating its thematic content, style, or audience appeal."@en ,
                        "Specifies the genre or category of a show, indicating its thematic content, style, or audience appeal." ;
           rdfs:label "has genre"@en ,
                      "has genre" .


###  http://ontology.show-catalog.org/show#/Has_rating
:Has_rating rdf:type owl:ObjectProperty ,
                     owl:AsymmetricProperty ,
                     owl:IrreflexiveProperty ;
            rdfs:domain :Show ;
            rdfs:range :Rating ;
            rdfs:comment "Specifies the rating assigned to a show, indicating its quality, content, or audience suitability."@en ,
                         "Specifies the rating assigned to a show, indicating its quality, content, or audience suitability." ;
            rdfs:label "has rating"@en ,
                       "has rating" .


###  http://ontology.show-catalog.org/show#/Participed_in
:Participed_in rdf:type owl:ObjectProperty ,
                        owl:AsymmetricProperty ,
                        owl:IrreflexiveProperty ;
               rdfs:domain :Person ;
               rdfs:range :Show ;
               rdfs:comment "Denotes a show in which a person has been involved, either as an actor, director, or in another role."@en ,
                            "Denotes a show in which a person has been involved, either as an actor, director, or in another role." ;
               rdfs:label "participated in"@en ,
                          "participated in" .


###  http://ontology.show-catalog.org/show#/Produced_in
:Produced_in rdf:type owl:ObjectProperty ,
                      owl:AsymmetricProperty ,
                      owl:IrreflexiveProperty ;
             rdfs:domain :Show ;
             rdfs:range :Country ;
             rdfs:comment "Specifies the country in which a show was produced, indicating the location or origin of the production process."@en ,
                          "Specifies the country in which a show was produced, indicating the location or origin of the production process." ;
             rdfs:label "produced in"@en ,
                        "produced in" .


#################################################################
#    Data properties
#################################################################

###  http://ontology.show-catalog.org/show#/MPAFilmRating
:MPAFilmRating rdf:type owl:DatatypeProperty ;
               rdfs:subPropertyOf :ratingLevel ;
               rdfs:domain :Rating ;
               rdfs:range xsd:string ;
               rdfs:comment "The Motion Picture Association film rating system is used in the United States and its territories to rate a motion picture's suitability for certain audiences based on its content. The system and the ratings applied to individual motion pictures are the responsibility of the Motion Picture Association (MPA). (source: https://www.motionpictures.org/film-ratings/)"@en ,
                            "The Motion Picture Association film rating system is used in the United States and its territories to rate a motion picture's suitability for certain audiences based on its content. The system and the ratings applied to individual motion pictures are the responsibility of the Motion Picture Association (MPA). (source: https://www.motionpictures.org/film-ratings/)" ;
               rdfs:label "MPA film rating system"@en ,
                          "MPA film rating system" .


###  http://ontology.show-catalog.org/show#/TVParentalGuidelines
:TVParentalGuidelines rdf:type owl:DatatypeProperty ;
                      rdfs:subPropertyOf :ratingLevel ;
                      rdfs:domain :Rating ;
                      rdfs:range xsd:string ;
                      rdfs:comment "The TV Parental Guidelines are a television content rating system in the United States. (source: https://en.wikipedia.org/wiki/TV_Parental_Guidelines)"@en ,
                                   "The TV Parental Guidelines are a television content rating system in the United States. (source: https://en.wikipedia.org/wiki/TV_Parental_Guidelines)" ;
                      rdfs:label "TV Parental Guidelines"@en ,
                                 "TV Parental Guidelines" .


###  http://ontology.show-catalog.org/show#/additionDate
:additionDate rdf:type owl:DatatypeProperty ;
              rdfs:domain :Show ;
              rdfs:range xsd:dateTime ;
              rdfs:comment "Specifies the date when a show was added or uploaded to a platform or database."@en ,
                           "Specifies the date when a show was added or uploaded to a platform or database." ;
              rdfs:label "addition date"@en ,
                         "addition date" .


###  http://ontology.show-catalog.org/show#/countryCode
:countryCode rdf:type owl:DatatypeProperty ;
             rdfs:domain :Country ;
             rdfs:range xsd:string ;
             rdfs:comment "The international Standard for country codes and codes for their subdivisions (ISO 3166) defines internationally recognized codes of letters and/or numbers that can be used when refering to countries and their subdivisions. (source : https://www.iso.org/iso-3166-country-codes.htmls)"@en ,
                          "The international Standard for country codes and codes for their subdivisions (ISO 3166) defines internationally recognized codes of letters and/or numbers that can be used when refering to countries and their subdivisions. (source : https://www.iso.org/iso-3166-country-codes.htmls)" ;
             rdfs:label "country code"@en ,
                        "country code" .


###  http://ontology.show-catalog.org/show#/duration
:duration rdf:type owl:DatatypeProperty ;
          rdfs:domain :Movie ;
          rdfs:range xsd:nonNegativeInteger ;
          rdfs:comment "Specifies the length of time in minutes for a movie's runtime or duration."@en ,
                       "Specifies the length of time in minutes for a movie's runtime or duration." ;
          rdfs:label "duration"@en ,
                     "duration" .


###  http://ontology.show-catalog.org/show#/name
:name rdf:type owl:DatatypeProperty ;
      rdfs:domain owl:Thing ;
      rdfs:range xsd:string ;
      rdfs:comment "Represents the name of a thing, providing the full textual name or label associated with that specific thing."@en ,
                   "Represents the name of a thing, providing the full textual name or label associated with that specific thing." ;
      rdfs:label "name"@en ,
                 "name" .


###  http://ontology.show-catalog.org/show#/numberOfSeasons
:numberOfSeasons rdf:type owl:DatatypeProperty ;
                 rdfs:domain :Series ;
                 rdfs:range xsd:nonNegativeInteger ;
                 rdfs:comment "Specifies the total number of seasons that a series comprises."@en ,
                              "Specifies the total number of seasons that a series comprises." ;
                 rdfs:label "number of seasons"@en ,
                            "number of seasons" .


###  http://ontology.show-catalog.org/show#/ratingLevel
:ratingLevel rdf:type owl:DatatypeProperty ;
             rdfs:domain :Rating ;
             rdfs:range xsd:string ;
             rdfs:comment "Represents the level or category of a rating, indicating classification of a show."@en ,
                          "Represents the level or category of a rating, indicating classification of a show." ;
             rdfs:label "rating level"@en ,
                        "rating level" .


###  http://ontology.show-catalog.org/show#/releaseYear
:releaseYear rdf:type owl:DatatypeProperty ;
             rdfs:domain :Show ;
             rdfs:range xsd:nonNegativeInteger ;
             rdfs:comment "Specifies the year when a show was released or made available to the public."@en ,
                          "Specifies the year when a show was released or made available to the public." ;
             rdfs:label "release year"@en ,
                        "release year" .


#################################################################
#    Classes
#################################################################

###  http://ontology.show-catalog.org/show#/Actor
:Actor rdf:type owl:Class ;
       rdfs:subClassOf :Person ;
       rdfs:comment "An actor or actress is a person who portrays a character in a production. (source: https://en.wikipedia.org/wiki/Actor)"@en ,
                    "An actor or actress is a person who portrays a character in a production. (source: https://en.wikipedia.org/wiki/Actor)" ;
       rdfs:label "Actor"@en ,
                  "Actor" .


###  http://ontology.show-catalog.org/show#/Country
:Country rdf:type owl:Class ;
         rdfs:subClassOf [ rdf:type owl:Restriction ;
                           owl:onProperty :name ;
                           owl:someValuesFrom xsd:string
                         ] ;
         rdfs:comment "A country is a distinct part of the world, such as a state, nation, or other political entity. When referring to a specific polity, the term \"country\" may refer to a sovereign state, states with limited recognition, constituent country, or a dependent territory. (source: https://en.wikipedia.org/wiki/Country)"@en ,
                      "A country is a distinct part of the world, such as a state, nation, or other political entity. When referring to a specific polity, the term \"country\" may refer to a sovereign state, states with limited recognition, constituent country, or a dependent territory. (source: https://en.wikipedia.org/wiki/Country)" ;
         rdfs:label "Country"@en ,
                    "Country" .


###  http://ontology.show-catalog.org/show#/Director
:Director rdf:type owl:Class ;
          rdfs:subClassOf :Person ;
          rdfs:comment "A film director is a person who controls a film's artistic and dramatic aspects and visualizes the screenplay (or script) while guiding the film crew and actors in the fulfillment of that vision. (source: https://en.wikipedia.org/wiki/Film_director)"@en ,
                       "A film director is a person who controls a film's artistic and dramatic aspects and visualizes the screenplay (or script) while guiding the film crew and actors in the fulfillment of that vision. (source: https://en.wikipedia.org/wiki/Film_director)" ;
          rdfs:label "Director"@en ,
                     "Director" .


###  http://ontology.show-catalog.org/show#/Genre
:Genre rdf:type owl:Class ;
       rdfs:subClassOf [ rdf:type owl:Restriction ;
                         owl:onProperty :name ;
                         owl:someValuesFrom xsd:string
                       ] ;
       rdfs:comment "A film genre is a stylistic or thematic category for motion pictures based on similarities either in the narrative elements, aesthetic approach, or the emotional response to the film. (source: https://en.wikipedia.org/wiki/Film_genre)"@en ,
                    "A film genre is a stylistic or thematic category for motion pictures based on similarities either in the narrative elements, aesthetic approach, or the emotional response to the film. (source: https://en.wikipedia.org/wiki/Film_genre)" ;
       rdfs:label "Genre"@en ,
                  "Genre" .


###  http://ontology.show-catalog.org/show#/Movie
:Movie rdf:type owl:Class ;
       rdfs:subClassOf :Show ;
       owl:disjointWith :Series ;
       rdfs:comment "A movie is a show where the full storyline is presented in one continuous film."@en ,
                    "A movie is a show where the full storyline is presented in one continuous film." ;
       rdfs:label "Movie"@en ,
                  "Movie" .


###  http://ontology.show-catalog.org/show#/Person
:Person rdf:type owl:Class ;
        rdfs:subClassOf [ rdf:type owl:Restriction ;
                          owl:onProperty :name ;
                          owl:someValuesFrom xsd:string
                        ] ;
        rdfs:comment "A person is a being who has certain capacities or attributes such as reason, morality, consciousness or self-consciousness, and being a part of a culturally established form of social relations such as kinship, ownership of property, or legal responsibility. (source: https://en.wikipedia.org/wiki/Person)"@en ,
                     "A person is a being who has certain capacities or attributes such as reason, morality, consciousness or self-consciousness, and being a part of a culturally established form of social relations such as kinship, ownership of property, or legal responsibility. (source: https://en.wikipedia.org/wiki/Person)" ;
        rdfs:label "Person"@en ,
                   "Person" .


###  http://ontology.show-catalog.org/show#/Rating
:Rating rdf:type owl:Class ;
        rdfs:subClassOf [ rdf:type owl:Restriction ;
                          owl:onProperty :ratingLevel ;
                          owl:someValuesFrom xsd:string
                        ] ;
        rdfs:comment "A content rating rates the suitability of TV shows, movies, comic books, or video games to this primary targeted audience. (source: https://en.wikipedia.org/wiki/Content_rating)"@en ,
                     "A content rating rates the suitability of TV shows, movies, comic books, or video games to this primary targeted audience. (source: https://en.wikipedia.org/wiki/Content_rating)" ;
        rdfs:label "Rating"@en ,
                   "Rating" .


###  http://ontology.show-catalog.org/show#/Series
:Series rdf:type owl:Class ;
        rdfs:subClassOf :Show ;
        rdfs:comment "A series is a show where the full storyline is divided into multiple film called episodes."@en ,
                     "A series is a show where the full storyline is divided into multiple film called episodes." ;
        rdfs:label "Series"@en ,
                   "Series" .


###  http://ontology.show-catalog.org/show#/Show
:Show rdf:type owl:Class ;
      rdfs:subClassOf [ rdf:type owl:Restriction ;
                        owl:onProperty :HasAsDirector ;
                        owl:someValuesFrom owl:Thing
                      ] ,
                      [ rdf:type owl:Restriction ;
                        owl:onProperty :Has_genre ;
                        owl:someValuesFrom owl:Thing
                      ] ,
                      [ rdf:type owl:Restriction ;
                        owl:onProperty :Produced_in ;
                        owl:someValuesFrom owl:Thing
                      ] ,
                      [ rdf:type owl:Restriction ;
                        owl:onProperty :name ;
                        owl:someValuesFrom xsd:string
                      ] ;
      rdfs:comment "A show is a visual or audio-visual production."@en ,
                   "A show is a visual or audio-visual production." ;
      rdfs:label "Show"@en ,
                 "Show" .


###  Generated by the OWL API (version 4.5.26.2023-07-17T20:34:13Z) https://github.com/owlcs/owlapi
